feat(super/splitting): split clauses into components

super/splitting.lean
@@ -1,7 +1,31 @@
 import .prover_state
-open monad
+open monad expr list tactic
 
 namespace super
+
+private meta def find_components : list expr → list (list (expr × ℕ)) → list (list (expr × ℕ))
+| (e::es) comps :=
+  let (contain_e, do_not_contain_e) :=
+      partition (λc : list (expr × ℕ), c↣exists_ $ λf,
+        (abstract_local f↣1 e↣local_uniq_name)↣has_var) comps in
+    find_components es $ list.join contain_e :: do_not_contain_e
+| _ comps := comps
+
+meta def get_components (hs : list expr) : list (list expr) :=
+(find_components hs (hs↣zip_with_index↣for $ λh, [h]))↣for $ λc,
+(sort_on (λh : expr × ℕ, h↣2) c)↣for $ λh, h↣1
+
+example (i : Type) (p q : i → Prop) (H : ∀x y, p x → q y → false) : true := by do
+h ← get_local `H >>= clause.of_proof,
+(op, lcs) ← h↣open_constn h↣num_binders,
+guard $ (get_components lcs)↣length = 2,
+triv
+
+example (i : Type) (p : i → i → Prop) (H : ∀x y z, p x y → p y z → false) : true := by do
+h ← get_local `H >>= clause.of_proof,
+(op, lcs) ← h↣open_constn h↣num_binders,
+guard $ (get_components lcs)↣length = 1,
+triv
 
 meta def extract_assertions : clause → resolution_prover (clause × list expr) | c :=
 if c↣num_lits = 0 then return (c, [])
@@ -22,37 +46,27 @@ else do
       return (op_wo_as↣1↣close_const op↣2, op_wo_as↣2)
   end
 
-meta def splitting_inf : inference := take given,
-if given↣c↣num_lits ≤ 1 then return () else do
-forM given↣c↣get_lits (λl,
-     if l↣formula↣has_var ∨ l↣formula↣is_not↣is_some then
-       return ()
-     else
-       mk_sat_var l↣formula l↣is_neg),
-with_ass ← extract_assertions given↣c,
-if with_ass↣2↣length > 0 then do
-  add_inferred with_ass↣1 [given],
-  remove_redundant given↣id []
-else
-  return ()
+meta def mk_splitting_clause' (orig_proof : expr) : list (list expr) → tactic (list expr × expr)
+| [] := return ([], orig_proof)
+| ([p] :: comps) := do p' : list expr × expr ← mk_splitting_clause' comps, return (p::p'↣1, p'↣2)
+| (comp :: comps) := do
+  (hs, p') ← mk_splitting_clause' comps,
+  hnc ← mk_local_def `hnc (pis comp false_)↣not_,
+  p'' ← return $ app hnc (lambdas comp p'),
+  return (hnc::hs, p'')
 
--- FIXME(gabriel): this introduces variables that are then not introduced as
--- clauses because they didn't change in the model...
-meta def splitting_pre : resolution_prover unit :=
-preprocessing_rule $ take news, do flip filterM news $ take new, do
-ass ← collect_ass_hyps new,
-if new↣num_quants = 0 ∧ new↣num_lits > 1 then do
-  add_sat_clause $ new↣close_constn ass,
-  return ff
-else if new↣num_quants = 0 ∧ new↣num_lits = 1 then do
-  hd ← return $ new↣get_lit 0,
-  hyp ← get_sat_hyp_core hd↣formula hd↣is_neg,
-  if hyp↣is_some then do
-    add_sat_clause $ new↣close_constn ass,
-    return ff
-  else
-    return tt
-else
-  return tt
+meta def mk_splitting_clause (orig_proof : expr) (comps : list (list expr)) : tactic clause := do
+(hs, p) ← mk_splitting_clause' orig_proof comps,
+return $ (clause.mk 0 0 p false_)↣close_constn hs
+
+meta def splitting_inf : inference := take given, do
+op : clause × list expr ← ↑(given↣c↣open_constn given↣c↣num_binders),
+if list.bor (given↣c↣get_lits↣for $ λl, l↣formula↣is_not↣is_some) then return () else
+let comps := get_components op↣2 in
+if comps↣length < 2 then return () else do
+splitting_clause ← ↑(mk_splitting_clause op↣1↣proof comps),
+ass ← collect_ass_hyps splitting_clause,
+add_sat_clause $ splitting_clause↣close_constn ass,
+remove_redundant given↣id []
 
 end super
